RocqOfRust/revm/revm_interpreter/instructions/simulate/bitwise.v
@@ -3,10 +3,12 @@ Require Import RocqOfRust.links.M.
 Require Import RocqOfRust.simulate.M.
 Require Import RocqOfRust.lib.simulate.lib.
 Require Import core.links.array.
+Require Import core.links.cmp.
 Require Import core.simulate.cmp.
 Require Import revm.revm_context_interface.links.host.
 Require Import revm.revm_interpreter.gas.simulate.constants.
 Require Import revm.revm_interpreter.instructions.links.bitwise.
+Require Import revm.revm_interpreter.instructions.simulate.i256.
 Require Import revm.revm_interpreter.instructions.simulate.macros.
 Require Import revm.revm_interpreter.links.gas.
 Require Import revm.revm_interpreter.links.interpreter.
@@ -70,9 +72,7 @@ Proof.
   popn_top_macro_eq InterpreterTypesEq.
   cbn.
   eapply Run.Call. {
-    setoid_rewrite (Impl_PartialOrd_for_Uint.Eq.I).(PartialOrd.Eq.lt).
-    get_can_access.
-    apply Run.Pure.
+    apply PartialOrd.Eq.lt; repeat unshelve econstructor.
   }
   cbn.
   eapply Run.Call. {
@@ -84,4 +84,215 @@ Proof.
   get_can_access.
   cbn.
   apply Run.PureEq; repeat f_equal.
+Qed.
+
+Definition gt
+    {WIRE : Set} `{Link WIRE}
+    {WIRE_types : InterpreterTypes.Types.t} `{InterpreterTypes.Types.AreLinks WIRE_types}
+    {IInterpreterTypes : InterpreterTypes.C WIRE_types}
+    (interpreter : Interpreter.t WIRE WIRE_types) :
+    Interpreter.t WIRE WIRE_types :=
+  gas_macro interpreter constants.VERYLOW id (fun interpreter =>
+  popn_top_macro interpreter {| Integer.value := 1 |} id (fun arr top interpreter =>
+    let '{| ArrayPair.x := op1 |} := arr.(array.value) in
+    let op2 := top.(RefStub.projection) interpreter.(Interpreter.stack) in
+    let result :=
+      if PartialOrd.gt op1 op2 then
+        {| Uint.value := 1 |}
+      else
+        {| Uint.value := 0 |} in
+    let stack :=
+      top.(RefStub.injection)
+        interpreter.(Interpreter.stack) result in
+    interpreter
+      <| Interpreter.stack := stack |>
+  )).
+
+Lemma gt_eq
+    {WIRE H : Set} `{Link WIRE} `{Link H}
+    {WIRE_types : InterpreterTypes.Types.t} `{InterpreterTypes.Types.AreLinks WIRE_types}
+    {H_types : Host.Types.t} `{Host.Types.AreLinks H_types}
+    (run_InterpreterTypes_for_WIRE : InterpreterTypes.Run WIRE WIRE_types)
+    (IInterpreterTypes : InterpreterTypes.C WIRE_types)
+    (InterpreterTypesEq :
+      InterpreterTypes.Eq.t WIRE WIRE_types run_InterpreterTypes_for_WIRE IInterpreterTypes)
+    (interpreter : Interpreter.t WIRE WIRE_types)
+    (_host : H) :
+  let ref_interpreter : '&mut (Interpreter.t WIRE WIRE_types) := make_ref 0 in
+  let ref_host : '&mut H := make_ref 1 in
+  {{
+    SimulateM.eval_f
+      (run_gt run_InterpreterTypes_for_WIRE ref_interpreter ref_host)
+      ([interpreter; _host]%stack) 🌲
+    (
+      Output.Success tt,
+      [
+        gt interpreter;
+        _host
+      ]%stack
+    )
+  }}.
+Proof.
+  intros.
+  unfold gt.
+  gas_macro_eq InterpreterTypesEq.
+  popn_top_macro_eq InterpreterTypesEq.
+  cbn.
+  eapply Run.Call. {
+    apply PartialOrd.Eq.gt; repeat unshelve econstructor.
+  }
+  cbn.
+  eapply Run.Call. {
+    apply Impl_Uint.from_eq.
+    { typeclasses eauto. }
+    { easy. }
+  }
+  cbn.
+  get_can_access.
+  cbn.
+  apply Run.PureEq; repeat f_equal.
+Qed.
+
+Definition slt
+    {WIRE : Set} `{Link WIRE}
+    {WIRE_types : InterpreterTypes.Types.t} `{InterpreterTypes.Types.AreLinks WIRE_types}
+    {IInterpreterTypes : InterpreterTypes.C WIRE_types}
+    (interpreter : Interpreter.t WIRE WIRE_types) :
+    Interpreter.t WIRE WIRE_types :=
+  gas_macro interpreter constants.VERYLOW id (fun interpreter =>
+  popn_top_macro interpreter {| Integer.value := 1 |} id (fun arr top interpreter =>
+    let '{| ArrayPair.x := op1 |} := arr.(array.value) in
+    let op2 := top.(RefStub.projection) interpreter.(Interpreter.stack) in
+    let result :=
+      match i256_cmp op1 op2 with
+      | Ordering.Less => {| Uint.value := 1 |}
+      | _ => {| Uint.value := 0 |}
+      end in
+    let stack :=
+      top.(RefStub.injection)
+        interpreter.(Interpreter.stack) result in
+    interpreter
+      <| Interpreter.stack := stack |>
+  )).
+
+Lemma slt_eq
+    {WIRE H : Set} `{Link WIRE} `{Link H}
+    {WIRE_types : InterpreterTypes.Types.t} `{InterpreterTypes.Types.AreLinks WIRE_types}
+    {H_types : Host.Types.t} `{Host.Types.AreLinks H_types}
+    (run_InterpreterTypes_for_WIRE : InterpreterTypes.Run WIRE WIRE_types)
+    (IInterpreterTypes : InterpreterTypes.C WIRE_types)
+    (InterpreterTypesEq :
+      InterpreterTypes.Eq.t WIRE WIRE_types run_InterpreterTypes_for_WIRE IInterpreterTypes)
+    (interpreter : Interpreter.t WIRE WIRE_types)
+    (_host : H) :
+  let ref_interpreter : '&mut (Interpreter.t WIRE WIRE_types) := make_ref 0 in
+  let ref_host : '&mut H := make_ref 1 in
+  {{
+    SimulateM.eval_f
+      (run_slt run_InterpreterTypes_for_WIRE ref_interpreter ref_host)
+      ([interpreter; _host]%stack) 🌲
+    (
+      Output.Success tt,
+      [
+        slt interpreter;
+        _host
+      ]%stack
+    )
+  }}.
+Proof.
+  intros.
+  unfold slt.
+  gas_macro_eq InterpreterTypesEq.
+  popn_top_macro_eq InterpreterTypesEq.
+  cbn.
+  eapply Run.Call. {
+    apply i256_cmp_eq; repeat unshelve econstructor.
+  }
+  cbn.
+  eapply Run.Call. {
+    apply PartialEq.Eq.eq; repeat unshelve econstructor.
+  }
+  cbn.
+  eapply Run.Call. {
+    apply Impl_Uint.from_eq.
+    { typeclasses eauto. }
+    { easy. }
+  }
+  cbn.
+  get_can_access.
+  cbn.
+  apply Run.PureEq; repeat f_equal.
+  now destruct i256_cmp.
+Qed.
+
+Definition sgt
+    {WIRE : Set} `{Link WIRE}
+    {WIRE_types : InterpreterTypes.Types.t} `{InterpreterTypes.Types.AreLinks WIRE_types}
+    {IInterpreterTypes : InterpreterTypes.C WIRE_types}
+    (interpreter : Interpreter.t WIRE WIRE_types) :
+    Interpreter.t WIRE WIRE_types :=
+  gas_macro interpreter constants.VERYLOW id (fun interpreter =>
+  popn_top_macro interpreter {| Integer.value := 1 |} id (fun arr top interpreter =>
+    let '{| ArrayPair.x := op1 |} := arr.(array.value) in
+    let op2 := top.(RefStub.projection) interpreter.(Interpreter.stack) in
+    let result :=
+      match i256_cmp op1 op2 with
+      | Ordering.Greater => {| Uint.value := 1 |}
+      | _ => {| Uint.value := 0 |}
+      end in
+    let stack :=
+      top.(RefStub.injection)
+        interpreter.(Interpreter.stack) result in
+    interpreter
+      <| Interpreter.stack := stack |>
+  )).
+
+Lemma sgt_eq
+    {WIRE H : Set} `{Link WIRE} `{Link H}
+    {WIRE_types : InterpreterTypes.Types.t} `{InterpreterTypes.Types.AreLinks WIRE_types}
+    {H_types : Host.Types.t} `{Host.Types.AreLinks H_types}
+    (run_InterpreterTypes_for_WIRE : InterpreterTypes.Run WIRE WIRE_types)
+    (IInterpreterTypes : InterpreterTypes.C WIRE_types)
+    (InterpreterTypesEq :
+      InterpreterTypes.Eq.t WIRE WIRE_types run_InterpreterTypes_for_WIRE IInterpreterTypes)
+    (interpreter : Interpreter.t WIRE WIRE_types)
+    (_host : H) :
+  let ref_interpreter : '&mut (Interpreter.t WIRE WIRE_types) := make_ref 0 in
+  let ref_host : '&mut H := make_ref 1 in
+  {{
+    SimulateM.eval_f
+      (run_sgt run_InterpreterTypes_for_WIRE ref_interpreter ref_host)
+      ([interpreter; _host]%stack) 🌲
+    (
+      Output.Success tt,
+      [
+        sgt interpreter;
+        _host
+      ]%stack
+    )
+  }}.
+Proof.
+  intros.
+  unfold sgt.
+  gas_macro_eq InterpreterTypesEq.
+  popn_top_macro_eq InterpreterTypesEq.
+  cbn.
+  eapply Run.Call. {
+    apply i256_cmp_eq; repeat unshelve econstructor.
+  }
+  cbn.
+  eapply Run.Call. {
+    apply PartialEq.Eq.eq; repeat unshelve econstructor.
+  }
+  cbn.
+  eapply Run.Call. {
+    apply Impl_Uint.from_eq.
+    { typeclasses eauto. }
+    { easy. }
+  }
+  cbn.
+  get_can_access.
+  cbn.
+  apply Run.PureEq; repeat f_equal.
+  now destruct i256_cmp.
 Qed.
