RocqOfRust/revm/revm_interpreter/instructions/simulate/i256.v
@@ -1,0 +1,94 @@
+Require Import RocqOfRust.RocqOfRust.
+Require Import RocqOfRust.links.M.
+Require Import RocqOfRust.simulate.M.
+Require Import alloy_primitives.links.aliases.
+Require Import core.links.cmp.
+Require Import core.simulate.cmp.
+Require Import revm.revm_interpreter.instructions.links.i256.
+Require Import ruint.links.lib.
+Require Import ruint.simulate.cmp.
+
+(*
+pub fn i256_sign(val: &U256) -> Sign {
+    if val.bit(U256::BITS - 1) {
+        Sign::Minus
+    } else {
+        // SAFETY: false == 0 == Zero, true == 1 == Plus
+        unsafe { core::mem::transmute::<bool, Sign>(!val.is_zero()) }
+    }
+}
+*)
+Definition i256_sign (val : aliases.U256.t) : Sign.t :=
+  let high_bit := Z.testbit val.(Uint.value) 255 in
+  if high_bit then
+    Sign.Minus
+  else if val.(Uint.value) =? 0 then
+    Sign.Zero
+  else
+    Sign.Plus.
+
+Lemma i256_sign_eq
+    (stack : Stack.t)
+    (ref_val : '& aliases.U256.t)
+    (val : aliases.U256.t) :
+  CanRead.t stack val ref_val ->
+  {{
+    SimulateM.eval_f
+      (run_i256_sign ref_val)
+      stack 🌲
+    (
+      Output.Success (i256_sign val),
+      stack
+    )
+  }}.
+Admitted.
+
+Module Impl_Ord_for_Sign.
+  Definition cmp (s1 s2 : Sign.t) : Ordering.t :=
+    match s1, s2 with
+    | Sign.Minus, Sign.Minus => Ordering.Equal
+    | Sign.Minus, _ => Ordering.Less
+    | Sign.Zero, Sign.Minus => Ordering.Greater
+    | Sign.Zero, Sign.Zero => Ordering.Equal
+    | Sign.Zero, Sign.Plus => Ordering.Less
+    | Sign.Plus, Sign.Plus => Ordering.Equal
+    | Sign.Plus, _ => Ordering.Greater
+    end.
+End Impl_Ord_for_Sign.
+
+(*
+pub fn i256_cmp(first: &U256, second: &U256) -> Ordering {
+    let first_sign = i256_sign(first);
+    let second_sign = i256_sign(second);
+    match first_sign.cmp(&second_sign) {
+        // Note: Adding `if first_sign != Sign::Zero` to short circuit zero comparisons performs
+        // slower on average, as of #582
+        Ordering::Equal => first.cmp(second),
+        o => o,
+    }
+}
+*)
+Definition i256_cmp (first second : aliases.U256.t) : Ordering.t :=
+  let first_sign := i256_sign first in
+  let second_sign := i256_sign second in
+  match Impl_Ord_for_Sign.cmp first_sign second_sign with
+  | Ordering.Equal => Impl_Ord_for_Uint.cmp first second
+  | o => o
+  end.
+
+Lemma i256_cmp_eq
+    (stack : Stack.t)
+    (ref_first ref_second : '& aliases.U256.t)
+    (first second : aliases.U256.t) :
+  CanRead.t stack first ref_first ->
+  CanRead.t stack second ref_second ->
+  {{
+    SimulateM.eval_f
+      (run_i256_cmp ref_first ref_second)
+      stack 🌲
+    (
+      Output.Success (i256_cmp first second),
+      stack
+    )
+  }}.
+Admitted.
